

Supplementary Material

Derivation of Taylor Series for erf

Recall the error function is defined as

$$\operatorname{erf}(x) := \frac{2}{\sqrt{\pi}} \int_0^x e^{-t^2} dt \quad (1)$$

The Taylor series expanded about $t = 0$ for e^{-t^2} is given as

$$e^{-t^2} = 1 - t^2 + \frac{t^4}{2} - \frac{t^6}{6} + \cdots = \sum_{k=0}^{\infty} (-1)^k \frac{t^{2k}}{k!} \quad (2)$$

The power series is uniformly convergent on \mathbb{R} , therefore it is also uniformly convergent on $[0, x]$. Using this fact to interchange the summation and integral we find

$$\begin{aligned} \int_0^x e^{-t^2} dt &= \int_0^x \left(\sum_{k=0}^{\infty} (-1)^k \frac{t^{2k}}{k!} \right) dt \\ &= \sum_{k=0}^{\infty} \frac{(-1)^k}{k!} \left(\int_0^x t^{2k} dt \right) \\ &= \sum_{k=0}^{\infty} \left[\frac{(-1)^k t^{2k+1}}{k!(2k+1)} \right]_0^x \\ &= \sum_{k=0}^{\infty} \frac{(-1)^k x^{2k+1}}{k!(2k+1)}. \end{aligned}$$

Thus, we arrive at the Taylor series for erf

$$\operatorname{erf}(x) = \frac{2}{\sqrt{\pi}} \sum_{k=0}^{\infty} \frac{(-1)^k x^{2k+1}}{k!(2k+1)}. \quad (3)$$

If we truncate the power series after the x^{2N+1} term, i.e. the upper limit of the summation is N , the first neglected term is

$$\frac{2}{\sqrt{\pi}} \frac{(-1)^{N+1} x^{2N+3}}{(N+1)!(2N+3)}. \quad (4)$$

For fixed $x > 0$, define

$$a_k(x) = \frac{x^{2k+1}}{k!(2k+1)} > 0. \quad (5)$$

Consider the ratio

$$\frac{a_{k+1}(x)}{a_k(x)} = \frac{(2k+1)}{(k+1)(2k+3)} x^2. \quad (6)$$

Therefore if the condition

$$\frac{(2N+1)}{(N+1)(2N+3)} x^2 < 1, \quad (7)$$

the terms in the Taylor series for $k = N + 1, N + 2, \dots$ are alternating and decreasing so the absolute error is bounded by the first neglected term, i.e.

$$|\varepsilon_N(x)| \leq \frac{2}{\sqrt{\pi}} \frac{x^{2N+3}}{(N+1)!(2N+3)}. \quad (8)$$

This is automatically satisfied for small x , but N must be sufficiently large for larger x . In practice, the rounding error significantly outweighs the truncation error for larger x , so we can safely take this to be an upper bound for the truncation error in the regions that this series is applied, i.e. $x \lesssim 2$.

Padé Approximation

An alternative to the Taylor series is a rational approximation in which we approximate the function using the ratio of two polynomials. The $[m/n]$ Padé approximation to a function f is a rational function

$$r(x) = \frac{p_0 + p_1x + \dots + p_mx^m}{q_0 + q_1x + \dots + q_nx^n} [1]. \quad (9)$$

We set $q_0 = 1$, and the remaining $m + n + 1$ coefficients are chosen such that

$$f^{(k)}(0) = r^{(k)}(0) \quad \text{for } k = 0, 1, \dots, m + n [1]. \quad (10)$$

Equation (9) and (10) are equivalent to the expression

$$(a_0 + a_1x + \dots)(1 + q_1x + \dots + q_nx^n) - (p_0 + p_1x + \dots + p_mx^m) \quad (11)$$

having no terms of degree $\leq N := m + n$, where $\{a_k\}$ are the Taylor coefficients of f .

For convenience, we set $p_{m+1} = p_{m+2} = \dots = p_N = 0$ and $q_{n+1} = q_{n+2} = \dots = q_N = 0$.

The condition stated in Equation (11) can be written as the linear system

$$\sum_{i=0}^k a_i q_{k-i} = p_k, \quad k = 0, 1, \dots, N. \quad (12)$$

For $k = m + 1, m + 2, \dots, N$, $p_k = 0$, which gives

$$\sum_{j=1}^n a_{k-j} q_j = -a_k. \quad (13)$$

This is a system of n linear equations in n unknowns.

After using Equation (13) to find q_1, \dots, q_n , we can then use Equation (12) for $k = 0, 1, \dots, m$ to calculate p_0, \dots, p_m directly.

When tested on the error function against the Taylor series, Padé approximation perform equally well on small values of x and better for larger x . However, the method fails to achieve the desired accuracy of $10\varepsilon_{\text{mach}}$ beyond $x \approx 3$. Therefore we do not explore this approximation further.

Bibliography

- [1] Burden, R. L., Faires J. D., and Burden, A. M. (2015). Numerical Analysis. (10th ed). Cengage Learning.